Incorporate session reasoning in pk_auth.

nown.v
@@ -15,39 +15,33 @@ Section NOwn.
 Context `{!heapGS Σ}.
 Notation iProp := (iProp Σ).
 
-Class nownGS := {
-  nownGS_name : gname;
-}.
+Definition nown_token γ E : iProp :=
+  own γ (reservation_map_token E).
 
-Context `{!nownGS}.
-
-Definition nown_token E : iProp :=
-  own nownGS_name (reservation_map_token E).
-
-Definition nown_name N (γ : gname) : iProp :=
-  own nownGS_name (namespace_map_data N (to_agree γ)).
+Definition nown_name γ N (γ' : gname) : iProp :=
+  own γ (namespace_map_data N (to_agree γ')).
 
 #[global]
-Instance nown_name_timeless N γ : Timeless (nown_name N γ).
+Instance nown_name_timeless γ N γ' : Timeless (nown_name γ N γ').
 Proof. apply _. Qed.
 
 #[global]
-Instance nown_name_persistent N γ : Persistent (nown_name N γ).
+Instance nown_name_persistent γ N γ' : Persistent (nown_name γ N γ').
 Proof. apply _. Qed.
 
-Lemma nown_name_set E N γ :
+Lemma nown_name_set E γ N γ' :
   ↑N ⊆ E →
-  nown_token E ==∗ nown_name N γ.
+  nown_token γ E ==∗ nown_name γ N γ'.
 Proof.
 iIntros (?) "token".
 iMod (own_update with "token") as "data".
-  by apply (namespace_map_alloc_update _ N (to_agree γ)).
+  by apply (namespace_map_alloc_update _ N (to_agree γ')).
 by eauto.
 Qed.
 
-Lemma nown_name_agree N γ1 γ2 :
-  nown_name N γ1 -∗
-  nown_name N γ2 -∗
+Lemma nown_name_agree γ N γ1 γ2 :
+  nown_name γ N γ1 -∗
+  nown_name γ N γ2 -∗
   ⌜γ1 = γ2⌝.
 Proof.
 iIntros "own1 own2".
@@ -56,75 +50,74 @@ move: valid; rewrite -reservation_map_data_op reservation_map_data_valid.
 by move=> /to_agree_op_inv_L ->.
 Qed.
 
-Lemma nown_token_difference E1 E2 :
+Lemma nown_token_difference γ E1 E2 :
   E1 ⊆ E2 →
-  nown_token E2 ⊣⊢ nown_token E1 ∗ nown_token (E2 ∖ E1).
+  nown_token γ E2 ⊣⊢ nown_token γ E1 ∗ nown_token γ (E2 ∖ E1).
 Proof.
 move=> ?.
 by rewrite /nown_token -own_op -reservation_map_token_difference.
 Qed.
 
-Definition nown `{!inG Σ A} N (a : A) : iProp :=
-  ∃ γ, nown_name N γ ∧ own γ a.
+Definition nown `{!inG Σ A} γ N (a : A) : iProp :=
+  ∃ γ', nown_name γ N γ' ∧ own γ' a.
 
-Lemma nown_alloc `{!inG Σ A} N E (a : A) :
-  ↑N ⊆ E → ✓ a → nown_token E ==∗ nown N a.
+Lemma nown_alloc `{!inG Σ A} γ N E (a : A) :
+  ↑N ⊆ E → ✓ a → nown_token γ E ==∗ nown γ N a.
 Proof.
 intros sub valid_a. iIntros "token".
-iMod (own_alloc a) as "(%γ & own)"; auto.
-iMod (nown_name_set γ with "token") as "name"; eauto.
-iModIntro. iExists γ. eauto.
+iMod (own_alloc a) as "(%γ' & own)"; auto.
+iMod (nown_name_set _ γ' with "token") as "name"; eauto.
+iModIntro. iExists γ'. eauto.
 Qed.
 
-Lemma nown_valid `{!inG Σ A} N (a : A) : nown N a -∗ ✓ a.
+Lemma nown_valid `{!inG Σ A} γ N (a : A) : nown γ N a -∗ ✓ a.
 Proof.
-iIntros "(%γ & #own_γ & own)". iApply (own_valid with "own").
+iIntros "(%γ' & #own_γ' & own)". iApply (own_valid with "own").
 Qed.
 
-Lemma nown_valid_2 `{!inG Σ A} N (a1 a2 : A) :
-  nown N a1 -∗ nown N a2 -∗ ✓ (a1 ⋅ a2).
+Lemma nown_valid_2 `{!inG Σ A} γ N (a1 a2 : A) :
+  nown γ N a1 -∗ nown γ N a2 -∗ ✓ (a1 ⋅ a2).
 Proof.
-iIntros "(%γ & #own_γ & own1) (%γ' & own_γ' & own2)".
-iPoseProof (nown_name_agree with "own_γ own_γ'") as "<-".
+iIntros "(%γ1 & #own_γ1 & own1) (%γ2 & own_γ2 & own2)".
+iPoseProof (nown_name_agree with "own_γ1 own_γ2") as "<-".
 by iApply (own_valid_2 with "own1 own2").
 Qed.
 
-Lemma nown_update `{!inG Σ A} N (a a' : A) : a ~~> a' → nown N a ==∗ nown N a'.
+Lemma nown_update `{!inG Σ A} γ N (a a' : A) :
+  a ~~> a' → nown γ N a ==∗ nown γ N a'.
 Proof.
-iIntros (?) "(%γ & #? & own)".
+iIntros (?) "(%γ' & #? & own)".
 iMod (own_update with "own") as "own"; eauto.
-iModIntro. iExists γ. eauto.
+iModIntro. iExists γ'. eauto.
 Qed.
 
 #[global]
-Instance nown_core_persistent `{!inG Σ A} N (a : A) :
-  CoreId a → Persistent (nown N a).
+Instance nown_core_persistent `{!inG Σ A} γ N (a : A) :
+  CoreId a → Persistent (nown γ N a).
 Proof. apply _. Qed.
 
 #[global]
-Instance nown_timeless `{!inG Σ A} N (a : A) :
-  Discrete a → Timeless (nown N a).
+Instance nown_timeless `{!inG Σ A} γ N (a : A) :
+  Discrete a → Timeless (nown γ N a).
 Proof. apply _. Qed.
 
-Lemma nown_op `{!inG Σ A} N (a1 a2 : A) :
-  nown N (a1 ⋅ a2) ⊣⊢ nown N a1 ∗ nown N a2.
+Lemma nown_op `{!inG Σ A} γ N (a1 a2 : A) :
+  nown γ N (a1 ⋅ a2) ⊣⊢ nown γ N a1 ∗ nown γ N a2.
 Proof.
 iSplit.
-- iIntros "(%γ & #? & [own1 own2])".
-  by iSplitL "own1"; iExists γ; iSplit.
-- iIntros "[(%γ & #own_γ & own1) (%γ' & #own_γ' & own2)]".
-  iPoseProof (nown_name_agree with "own_γ own_γ'") as "<-".
-  iExists γ. iSplit => //. by iSplitL "own1".
+- iIntros "(%γ' & #? & [own1 own2])".
+  by iSplitL "own1"; iExists γ'; iSplit.
+- iIntros "[(%γ1 & #own_γ1 & own1) (%γ2 & #own_γ2 & own2)]".
+  iPoseProof (nown_name_agree with "own_γ1 own_γ2") as "<-".
+  iExists γ1. iSplit => //. by iSplitL "own1".
 Qed.
 
 End NOwn.
 
-Lemma nownGS_alloc `{!heapGS Σ} : ⊢ |==> ∃ (H : nownGS), nown_token ⊤.
+Lemma nownGS_alloc `{!heapGS Σ} : ⊢ |==> ∃ γ , nown_token γ ⊤.
 Proof.
-iMod (own_alloc (reservation_map_token ⊤)) as "(%γ & own)".
-  apply reservation_map_token_valid.
-iModIntro.
-by iExists (Build_nownGS γ).
+iApply (own_alloc (reservation_map_token ⊤)).
+apply reservation_map_token_valid.
 Qed.
 
-Arguments nown_alloc {Σ _ _ A _} N {_} a.
+Arguments nown_alloc {Σ _ A _} γ N {_} a.
